combined few tests

Test/dafny0/Trait/TraitOverride1.dfy
@@ -1,6 +1,7 @@
 // RUN: %dafny /compile:0 /print:"%t.print" /dprint:"%t.dprint" "%s" > "%t"
 // RUN: %diff "%s.expect" "%t"
 
+//everything should work OK in this test file
 trait T1
 {
    function method Plus (x:int, y:int) : int
@@ -52,3 +53,142 @@ class C1 extends T1
    }
 }
 
+trait T2 
+{
+	function method F(x: int): int
+	requires x < 100;
+	ensures F(x) < 100;
+	
+	method M(x: int) returns (y: int)
+	requires 0 <= x;
+	ensures x < y;
+}
+
+class C2 extends T2 
+{
+	function method F(x: int): int
+	requires x < 100;
+	ensures F(x) < 100;
+	{
+	   x
+	}
+	
+	method M(x: int) returns (y: int)
+	requires -2000 <= x; // a more permissive precondition than in the interface
+	ensures 2*x < y; // a more detailed postcondition than in the interface
+	{
+	   y := (2 * x) + 1;
+	}
+}
+
+
+trait T3 
+{
+	function method F(y: int): int
+	function method G(y: int): int { 12 }
+	method M(y: int)
+	method N(y: int) {  
+           var a:int := 100;
+	   assert a==100;
+	}
+}
+class C3 extends T3
+{
+	function method NewFunc (a:int, b:int) : int
+	{
+	    a + b
+	}
+	function method F(y: int): int { 20 }
+	method M(y: int) { 
+	   var a:int := 100;
+	   assert a==100;
+	}
+}
+
+trait t
+{
+  function f(s2:int):int
+  ensures f(s2) > 0;
+  //requires s != null && s.Length > 1;
+  //reads s, s2;
+}
+
+class c extends t
+{
+  function f(s3:int):int
+  ensures f(s3) > 1;
+  //requires s0 != null && s0.Length > (0);
+  //reads s0;
+  { 
+     2
+  }
+}
+
+trait P1
+{
+  method M(N: int, a: array<int>) returns (sum: int)
+  {
+    sum := 1;   
+  }
+}
+
+class CC1 extends P1
+{
+
+}
+
+trait TT
+{
+   static function method M(a:int, b:int) : int
+     ensures M(a,b) == a + b;
+   {
+       a + b
+   }
+}
+
+class CC extends TT 
+{
+   method Testing(a:int,b:int)
+   {
+       assert (TT.M(a,b) == a + b);
+   }
+}
+
+
+trait T4 
+{
+	function method F(y: int): int
+	
+	function method G(y: int): int 
+	{ 
+	   100 
+	}
+	
+	method M(y: int) returns (kobra:int)
+	  requires y > 0;
+	  ensures kobra > 0;
+	   
+	method N(y: int) 
+	{ 
+	   var x: int;
+	   var y : int;
+	   y := 10;
+	   x := 1000;
+	   y := y + x;
+	}
+}
+
+class C4 extends T4 
+{
+	function method F(y: int): int 
+	{ 
+	  200 
+	}
+
+	method M(kk:int) returns (ksos:int)
+	  requires kk > (-1);
+	  ensures ksos > 0;
+	{
+		ksos:=10;	
+	}	 
+}
